p256: add constants for base point

code/ecdsap256/Hacl.Impl.P256.Constants.fst
@@ -49,7 +49,6 @@ let make_order n =
   bn_make_u64_4 n0 n1 n2 n3 n
 
 
-inline_for_extraction noextract
 val make_a_coeff: a:felem -> Stack unit
   (requires fun h -> live h a)
   (ensures fun h0 _ h1 -> modifies (loc a) h0 h1 /\
@@ -57,6 +56,7 @@ val make_a_coeff: a:felem -> Stack unit
     SM.fromDomain_ (as_nat h1 a) == S.a_coeff /\
     as_nat h1 a < S.prime)
 
+[@CInline]
 let make_a_coeff a =
   // a_coeff      = 0xffffffff00000001000000000000000000000000fffffffffffffffffffffffc
   // a_coeff_mont = 0xfffffffc00000004000000000000000000000003fffffffffffffffffffffffc
@@ -71,7 +71,6 @@ let make_a_coeff a =
   bn_make_u64_4 n0 n1 n2 n3 a
 
 
-inline_for_extraction noextract
 val make_b_coeff: b:felem -> Stack unit
   (requires fun h -> live h b)
   (ensures fun h0 _ h1 -> modifies (loc b) h0 h1 /\
@@ -79,6 +78,7 @@ val make_b_coeff: b:felem -> Stack unit
     SM.fromDomain_ (as_nat h1 b) == S.b_coeff /\
     as_nat h1 b < S.prime)
 
+[@CInline]
 let make_b_coeff b =
   // b_coeff      = 0x5ac635d8aa3a93e7b3ebbd55769886bc651d06b0cc53b0f63bce3c3e27d2604b
   // b_coeff_mont = 0xdc30061d04874834e5a220abf7212ed6acf005cd78843090d89cdf6229c4bddf
@@ -92,6 +92,43 @@ let make_b_coeff b =
     SM.fromDomain_ (v n0 + v n1 * pow2 64 + v n2 * pow2 128 + v n3 * pow2 192) == S.b_coeff);
   bn_make_u64_4 n0 n1 n2 n3 b
 
+
+val make_g_x: n:felem -> Stack unit
+  (requires fun h -> live h n)
+  (ensures  fun h0 _ h1 -> modifies (loc n) h0 h1 /\
+    as_nat h1 n == SM.toDomain_ S.g_x /\
+    SM.fromDomain_ (as_nat h1 n) == S.g_x)
+
+[@CInline]
+let make_g_x n =
+  // g_x = 0x6B17D1F2E12C4247F8BCE6E563A440F277037D812DEB33A0F4A13945D898C296
+  // mont_g_x = 0x18905f76a53755c679fb732b7762251075ba95fc5fedb60179e730d418a9143c
+  [@inline_let] let n0 = u64 0x79e730d418a9143c in
+  [@inline_let] let n1 = u64 0x75ba95fc5fedb601 in
+  [@inline_let] let n2 = u64 0x79fb732b77622510 in
+  [@inline_let] let n3 = u64 0x18905f76a53755c6 in
+  assert_norm (v n0 + v n1 * pow2 64 + v n2 * pow2 128 + v n3 * pow2 192 == SM.toDomain_ S.g_x);
+  assert_norm (SM.fromDomain_ (v n0 + v n1 * pow2 64 + v n2 * pow2 128 + v n3 * pow2 192) == S.g_x);
+  bn_make_u64_4 n0 n1 n2 n3 n
+
+
+val make_g_y: n:felem -> Stack unit
+  (requires fun h -> live h n)
+  (ensures  fun h0 _ h1 -> modifies (loc n) h0 h1 /\
+    as_nat h1 n == SM.toDomain_ S.g_y /\
+    SM.fromDomain_ (as_nat h1 n) == S.g_y)
+
+[@CInline]
+let make_g_y n =
+  // g_y = 0x4FE342E2FE1A7F9B8EE7EB4A7C0F9E162BCE33576B315ECECBB6406837BF51F5
+  // mont_g_x = 0x8571ff1825885d85d2e88688dd21f3258b4ab8e4ba19e45cddf25357ce95560a
+  [@inline_let] let n0 = u64 0xddf25357ce95560a in
+  [@inline_let] let n1 = u64 0x8b4ab8e4ba19e45c in
+  [@inline_let] let n2 = u64 0xd2e88688dd21f325 in
+  [@inline_let] let n3 = u64 0x8571ff1825885d85 in
+  assert_norm (v n0 + v n1 * pow2 64 + v n2 * pow2 128 + v n3 * pow2 192 == SM.toDomain_ S.g_y);
+  assert_norm (SM.fromDomain_ (v n0 + v n1 * pow2 64 + v n2 * pow2 128 + v n3 * pow2 192) == S.g_y);
+  bn_make_u64_4 n0 n1 n2 n3 n
 
 //----------------
 
