code/ecdsap256/Hacl.Impl.P256.PointMul.fst
@@ -253,12 +253,12 @@ val montgomery_ladder: #buf_type: buftype->  p: point -> q: point ->
 
 
       (
-	let p1 = fromDomainPoint(point_prime_to_coordinates (as_seq h1 p)) in
-	let q1 = fromDomainPoint(point_prime_to_coordinates (as_seq h1 q)) in
+	let p1 = fromDomainPoint(as_point_nat (as_seq h1 p)) in
+	let q1 = fromDomainPoint(as_point_nat (as_seq h1 q)) in
 	let rN, qN = S.montgomery_ladder_spec (as_seq h0 scalar)
 	  (
-	    fromDomainPoint(point_prime_to_coordinates (as_seq h0 p)),
-	    fromDomainPoint(point_prime_to_coordinates (as_seq h0 q))
+	    fromDomainPoint(as_point_nat (as_seq h0 p)),
+	    fromDomainPoint(as_point_nat (as_seq h0 q))
 	  ) in
 	rN == p1 /\ qN == q1
       )
@@ -274,7 +274,7 @@ let montgomery_ladder #a p q scalar tempBuffer =
 
   [@inline_let]
   let acc (h:mem) : GTot (tuple2 S.jacob_point S.jacob_point) =
-  (fromDomainPoint(point_prime_to_coordinates (as_seq h p)), fromDomainPoint(point_prime_to_coordinates (as_seq h q)))  in
+  (fromDomainPoint(as_point_nat (as_seq h p)), fromDomainPoint(as_point_nat (as_seq h q)))  in
 
   Lib.LoopCombinators.eq_repeati0 256 (spec_ml h0) (acc h0);
   [@inline_let]
@@ -305,18 +305,18 @@ val lemma_point_to_domain: h0: mem -> h1: mem ->  p: point -> result: point ->  
        point_z_as_nat h1 result == toDomain_ (point_z_as_nat h0 p)
      )
    )
-   (ensures (fromDomainPoint(point_prime_to_coordinates (as_seq h1 result)) == point_prime_to_coordinates (as_seq h0 p)))
+   (ensures (fromDomainPoint(as_point_nat (as_seq h1 result)) == as_point_nat (as_seq h0 p)))
 
 let lemma_point_to_domain h0 h1 p result =
-  let (x, y, z) = point_prime_to_coordinates (as_seq h1 result) in ()
+  let (x, y, z) = as_point_nat (as_seq h1 result) in ()
 
 
 val lemma_pif_to_domain: h: mem ->  p: point -> Lemma
   (requires (point_x_as_nat h p == 0 /\ point_y_as_nat h p == 0 /\ point_z_as_nat h p == 0))
-  (ensures (fromDomainPoint (point_prime_to_coordinates (as_seq h p)) == point_prime_to_coordinates (as_seq h p)))
+  (ensures (fromDomainPoint (as_point_nat (as_seq h p)) == as_point_nat (as_seq h p)))
 
 let lemma_pif_to_domain h p =
-  let (x, y, z) = point_prime_to_coordinates (as_seq h p) in
+  let (x, y, z) = as_point_nat (as_seq h p) in
   let (x3, y3, z3) = fromDomainPoint (x, y, z) in
   lemmaFromDomain x;
   lemmaFromDomain y;
@@ -327,7 +327,7 @@ let lemma_pif_to_domain h p =
 
 
 val lemma_coord: h3: mem -> q: point -> Lemma (
-   let (r0, r1, r2) = fromDomainPoint(point_prime_to_coordinates (as_seq h3 q)) in
+   let (r0, r1, r2) = fromDomainPoint(as_point_nat (as_seq h3 q)) in
 	let xD = fromDomain_ (point_x_as_nat h3 q) in
 	let yD = fromDomain_ (point_y_as_nat h3 q) in
 	let zD = fromDomain_ (point_z_as_nat h3 q) in
@@ -358,7 +358,7 @@ val scalarMultiplication_t: #t:buftype -> p: point -> result: point ->
     modifies (loc p |+| loc result |+| loc tempBuffer) h0 h1 /\
     (
       let x3, y3, z3 = point_x_as_nat h1 result, point_y_as_nat h1 result, point_z_as_nat h1 result in
-      let (xN, yN, zN) = S.scalar_multiplication (as_seq h0 scalar) (point_prime_to_coordinates (as_seq h0 p)) in
+      let (xN, yN, zN) = S.scalar_multiplication (as_seq h0 scalar) (as_point_nat (as_seq h0 p)) in
       x3 == xN /\ y3 == yN /\ z3 == zN
   )
 )
@@ -367,7 +367,7 @@ val scalarMultiplication_t: #t:buftype -> p: point -> result: point ->
 let scalarMultiplication_t #t p result scalar tempBuffer  =
     let h0 = ST.get() in
   let q = sub tempBuffer (size 0) (size 12) in
-  zero_buffer q;
+  make_point_at_inf q;
   let buff = sub tempBuffer (size 12) (size 88) in
   pointToDomain p result;
     let h2 = ST.get() in
@@ -395,7 +395,7 @@ let scalarMultiplication #buf_type p result scalar tempBuffer =
 let scalarMultiplicationWithoutNorm p result scalar tempBuffer =
   let h0 = ST.get() in
   let q = sub tempBuffer (size 0) (size 12) in
-  zero_buffer q;
+  make_point_at_inf q;
   let buff = sub tempBuffer (size 12) (size 88) in
   pointToDomain p result;
     let h2 = ST.get() in
@@ -409,10 +409,10 @@ let scalarMultiplicationWithoutNorm p result scalar tempBuffer =
 let secretToPublic result scalar tempBuffer =
   push_frame();
        let basePoint = create (size 12) (u64 0) in
-    uploadBasePoint basePoint;
+    make_base_point basePoint;
       let q = sub tempBuffer (size 0) (size 12) in
       let buff = sub tempBuffer (size 12) (size 88) in
-    zero_buffer q;
+    make_point_at_inf q;
       let h1 = ST.get() in
       lemma_pif_to_domain h1 q;
     montgomery_ladder q basePoint scalar buff;
@@ -423,10 +423,10 @@ let secretToPublic result scalar tempBuffer =
 let secretToPublicWithoutNorm result scalar tempBuffer =
     push_frame();
       let basePoint = create (size 12) (u64 0) in
-    uploadBasePoint basePoint;
+    make_base_point basePoint;
       let q = sub tempBuffer (size 0) (size 12) in
       let buff = sub tempBuffer (size 12) (size 88) in
-    zero_buffer q;
+    make_point_at_inf q;
       let h1 = ST.get() in
       lemma_pif_to_domain h1 q;
     montgomery_ladder q basePoint scalar buff;
